\begin{enumerate}
\item 
The cylcotron frequency will be given by
\begin{align*}
	\omega_c &= \frac{v}{r}
\end{align*}

In a cylcotron, the motion is given by
\begin{align*}
	\frac{mv^2}{r} &= qvB_0
\end{align*}
and so
\begin{align*}
	\frac{v}{r} &= \frac{q}{m}B_0
\end{align*}
Therefore
\begin{displaymath}
	\omega_c = \frac{q}{m}B_0
\end{displaymath}

\item At radius $r$, the particle will have velocity $v = \frac{q}{m}B_0 r$, and hence will have kinetic energy
\begin{align*}
	T &= \frac{1}{2}mv^2 \\
		&= \frac{1}{2}m \frac{q^2}{m^2}B_0^2r^2\\
		&= \frac{1}{2}\frac{q^2}{m}B_0^2r^2
\end{align*}

\item When the relativistic equation has to be used, we get that the velocity no longer increases as $\sqrt{T}$, but is given by
\begin{align*}
	T &= (\gamma - 1)mc^2\\
	\frac{T}{mc^2}+1 &= \frac{1}{\sqrt{1 - \left(\frac{v}{c}\right)^2}}\\
	\sqrt{1 - \left( \frac{v}{c}\right)^2} &= \frac{1}{\frac{T}{mc^2}+1}\\
	1 - \frac{v^2}{c^2} &= \left(\frac{1}{\frac{T}{mc^2}+1}\right)^2\\
	\frac{v^2}{c^2} &= 1 - \left(\frac{1}{\frac{T}{mc^2}+1}\right)^2\\
	v &= c\sqrt{1 - \left(\frac{1}{\frac{T}{mc^2}+1}\right)^2}
\end{align*}

Then, since $\omega_c \propto v$, and $v$ is no longer proportional to $r$, the cylcotron constant must vary with $v$.
\end{enumerate}